Start
(cherry-picked from b78bd1fd)

Strata/DL/Lambda/LState.lean
@@ -159,7 +159,7 @@ instance : ToFormat (T.Identifier × LState T) where
 /--
 Substitute `.fvar`s in `e` by looking up their values in `σ`.
 -/
-def LExpr.substFvarsFromState (σ : (LState T)) (e : (LExpr T.mono)) : (LExpr T.mono) :=
+@[expose] def LExpr.substFvarsFromState (σ : (LState T)) (e : (LExpr T.mono)) : (LExpr T.mono) :=
   let sm := σ.state.toSingleMap.map (fun (x, (_, v)) => (x, v))
   Lambda.LExpr.substFvars e sm
 
